\documentclass{article}
\usepackage{epsfig}
\usepackage{amsmath,amssymb}
\pagestyle{empty}
\begin{document}
$n$
\pagebreak

$M$
\pagebreak

$x_m$
\pagebreak

\[ y[n] = \sum_{m=0}^{M-1} x_m[n] \]
\pagebreak

\[ \mathbf{y}(k) = \mathbf{A} \mathbf{x}(k) \, , \, y \in \mathbb{R}^N, \mathbf{x} \in \mathbb{R}^M, A \in \mathbb{R}^{N \times M} \]
\pagebreak

$\mathbf{y}(k)$
\pagebreak

$\mathbf{x}(i)$
\pagebreak

$k$
\pagebreak

$\mathbf{A}$
\pagebreak

$l$
\pagebreak

$(A)_{l,k} \neq 0$
\pagebreak

$l \iff (A)_{l,k} \neq 0$
\pagebreak

$\lfloor N/2 \rfloor$
\pagebreak

$g(k)$
\pagebreak

$ \sum_{k=0}^{K-1} g(k) = 1$
\pagebreak

$ h \cdot \pi$
\pagebreak

\[ y[n] = exp (j 2 \pi \frac{f_{\Delta}}{f_s} \sum{x[n]}) \]
\pagebreak

$ f_{\Delta} $
\pagebreak

$f_s$
\pagebreak

\[ k = 2 \pi \frac{f_{\Delta}}{f_s} \]
\pagebreak

$y[n] = \mathrm{arg}\left(x[n] \, \bar x [n-1]\right)$
\pagebreak

$x$
\pagebreak

$A>0$
\pagebreak

$f\in\mathbb R$
\pagebreak

$\phi_0\in[0;2\pi]$
\pagebreak

$f_s>0$
\pagebreak

$x[n]= A e^{j2\pi( \frac f{f_s} n + \phi_0)}$
\pagebreak

\begin{align*} y[n] &= \mathrm{arg}\left(A e^{j2\pi\left( \frac f{f_s} n + \phi_0\right)} \overline{A e^{j2\pi( \frac f{f_s} (n-1) + \phi_0)}}\right)\\ & = \mathrm{arg}\left(A^2 e^{j2\pi\left( \frac f{f_s} n + \phi_0\right)} e^{-j2\pi( \frac f{f_s} (n-1) + \phi_0)}\right)\\ & = \mathrm{arg}\left( A^2 e^{j2\pi\left( \frac f{f_s} n + \phi_0 - \frac f{f_s} (n-1) - \phi_0\right)}\right)\\ & = \mathrm{arg}\left( A^2 e^{j2\pi\left( \frac f{f_s} n - \frac f{f_s} (n-1)\right)}\right)\\ & = \mathrm{arg}\left( A^2 e^{j2\pi\left( \frac f{f_s} \left(n-(n-1)\right)\right)}\right)\\ & = \mathrm{arg}\left( A^2 e^{j2\pi \frac f{f_s}}\right) \intertext{$A$ is real, so is $A^2$ and hence only \textit{scales}, therefore $\mathrm{arg}(\cdot)$ is invariant:} &= \mathrm{arg}\left(e^{j2\pi \frac f{f_s}}\right)\\ &= \frac f{f_s}\\ &&\blacksquare \end{align*}
\pagebreak

$c_i \in C$
\pagebreak

$s_i \in [00, 01, 10, 11]$
\pagebreak

$s_0$
\pagebreak

$c_0$
\pagebreak

$k_a)$
\pagebreak

$k_w$
\pagebreak

$k_a=1$
\pagebreak

$k_w=2$
\pagebreak

$k_a$
\pagebreak

$\hat{\varphi}$
\pagebreak

\[ M(d) = \frac{|P(d)|^2}{(R(d))^2}, \]
\pagebreak

\[ R(d) = \frac{1}{2} \sum_{k=0}^{N-1} |r_{k+d}|^2, \]
\pagebreak

$ x=G^T s $
\pagebreak

$\overline{x}$
\pagebreak

$\mathbf{H}\bar{x}^{T}=\overline{0}$
\pagebreak

$\mathbf{G}=\left[\mathbf{I}_{k}|\mathbf{P}\right]$
\pagebreak

$\mathbf{I}_{k}$
\pagebreak

$\mathbf{P}$
\pagebreak

$\bar{s}$
\pagebreak

\[\overline{x}=\mathbf{G}^{T}\bar{s}\]
\pagebreak

\[\left[\begin{array}{ccc} T & A & B\\ E & C & D \end{array}\right]\]
\pagebreak

\[ y[n] + \sum_{k=1}^{M} a_k y[n-k] = \sum_{k=0}^{N} b_k x[n-k] \]
\pagebreak

\[ H(z) = \frac{\sum_{k=0}^{N} b_k z^{-k}}{1 + \sum_{k=1}^{M} a_k z^{-k}} \]
\pagebreak

$y$
\pagebreak

$a_k$
\pagebreak

$b_k$
\pagebreak

$N$
\pagebreak

$a_0$
\pagebreak

\[ y[n] - \sum_{k=1}^{M} a_k y[n-k] = \sum_{k=0}^{N} b_k x[n-k] \]
\pagebreak

\[ H(z) = \frac{\sum_{k=0}^{M} b_k z^{-k}}{1 - \sum_{k=1}^{N} a_k z^{-k}} \]
\pagebreak

\end{document}
